# 2: Equations with Fractions

## Equation:

$$
(\frac{x-3}{4}+\frac{5-y}{2}=\frac{1}{4})\hspace{0.1cm}..X4..(1)
$$

$$
(\frac{2x-1}{3}-\frac{4+3}{2}=\frac{-13}{6})\hspace{0.1cm}..X6..(2)
$$

1. Get rid of LCD (Least Common Denominator)

$$
(\frac{\cancel{4}(x-3)}{\cancel{4}}+\frac{\cancel{4}\hspace{0.1cm}2(5-y)}{\cancel{2}}=\frac{\cancel{4}(1)}{\cancel{4}})\hspace{0.1cm}....(1)
$$

$$
\underline{(\frac{\cancel{6}\hspace{0.1cm}2(2x-1)}{\cancel{3}}+\frac{\cancel{6}\hspace{0.1cm}3(y+3)}{\cancel{2}}=\frac{\cancel{6}(-13)}{\cancel{6}})}\hspace{0.1cm}....(2)
$$

$$
x-3+10-2y=1\hspace{0.1cm}....(1)
$$

$$
x-2y=-6\hspace{0.1cm}....(1)
$$

$$
 
$$

$$
4x-2+3y+9=13\hspace{0.1cm}....(2)
$$

$$
4x+3y=-2\hspace{0.1cm}....(2)
$$

$$
 
$$

$$
x-2y=-6\hspace{0.1cm}..X-4..(1)
$$

$$
4x+3y=-2\hspace{0.1cm}....(2)
$$

$$
 
$$

$$
\cancel{-4x}+8y=24\hspace{0.1cm}....(1)
$$

$$
\cancel{4x}-3y=-2\hspace{0.1cm}....(2)
$$

$$
 
$$

$$
\frac{5y}{5}=\frac{22}{5}
$$

$$
y = 4.4
$$

$$
 
$$

$$
x-2y=-6\hspace{0.1cm}....(1)
$$

$$
x-2(4.4)=-6\hspace{0.1cm}....(1)
$$

$$
x=-6+2(4.4)
$$

$$
x=2.8
$$